L_Core_Infrastructure.v
@@ -790,10 +790,10 @@ Proof.
   -split; induction* Hp. 
    + pick_fresh y. forwards~ : (H0 y).
    + pick_fresh a.
-     destruct* (typing_regular_clos (E & a ~ T) c ).
+     destruct* (typing_regular_clos (E & a ~ neg T) c ).
    + apply_fresh proof_mu.
      rewrite open_clos_cont_def.
-     destruct* (typing_regular_clos (E & y~T) c).
+     destruct* (typing_regular_clos (E & y~neg T) c).
      rewrite* <- (@open_rec_clos_cont_id c (co_fvar y) H1 0).
   -split; induction* He.
     + pick_fresh a.
