L_Core_Soundness.v
@@ -1,0 +1,175 @@
+(***************************************************************************
+* Safety for Simply Typed Lambda Calculus (CBV) - Proofs                   *
+* Brian Aydemir & Arthur Chargueraud, July 2007                            *
+***************************************************************************)
+
+Set Implicit Arguments.
+Require Import LibLN 
+  L_Core_Definitions 
+  L_Core_Infrastructure.
+
+
+(* ********************************************************************** *)
+(** * Proofs *)
+
+(** Typing is preserved by weakening. *)
+
+Require Import Coq.Program.Equality.
+Scheme typing_prf_ind := Induction for typing_prf Sort Prop
+                         with typing_cont_ind := Induction for typing_cont Sort Prop
+                       with typing_clos_ind := Induction for typing_clos Sort Prop.
+About typing_clos_ind.
+
+Combined Scheme typing_mutind from typing_prf_ind,typing_cont_ind,typing_clos_ind.
+About typing_mutind.
+Lemma typing_weaken :
+  (  forall A p  T (H: A|= p :+ T) E F G,
+       A=E&G -> 
+       ok (E & F & G) ->  (E & F & G) |= p :+ T)
+/\ (forall A e T (H:(A) |= e :- T) E F G,
+A=E&G ->  ok (E & F & G) ->   (E & F & G) |= e :- T)
+/\ (forall A c  (H: (c:* A)) E F G,
+ A=E&G -> ok (E & F & G) ->   c:* (E & F & G)) .
+Proof.
+  apply (typing_mutind ).
+  + intros A a T OkA Binds E F G HA Ok.
+    apply* typing_prf_var. apply* binds_weaken.
+    rewrite HA in Binds.
+    assumption.
+  + intros L A U T p Ha IH E F G HA Ok.
+    apply_fresh typing_abs.
+    rewrite <- concat_assoc.
+    apply* IH.
+    rewrite HA.
+    rewrite <-concat_assoc.
+    reflexivity.
+    rewrite concat_assoc.
+    apply* ok_push.
+  + intros L A T c Ha IH E F G HA Ok.
+    apply_fresh (@typing_mu). 
+    rewrite <- concat_assoc.
+    apply* (IH y) .
+    rewrite HA.
+    rewrite <- concat_assoc.
+    reflexivity.
+    rewrite concat_assoc.
+    apply* ok_push.
+  + intros A a T OkA Binds E F G HA Ok.     
+    apply* typing_cont_var.
+    rewrite HA in Binds.
+    apply* binds_weaken.
+  + intros L A T c Ha IH E F G HA Ok.
+    apply_fresh typing_cont_mut.
+    rewrite <- concat_assoc.
+    apply* (IH y).
+    rewrite concat_assoc.
+    rewrite* HA.
+    rewrite concat_assoc.
+    apply* ok_push. 
+  + intros A U T q e Hq IHq He IHe E F G HA Ok.
+    apply* typing_stack.
+  + intros A T p e Hp IHp He IHe E F G HA Ok.
+    rewrite HA in *.
+    apply (@typing_closure (E&F&G) T); [apply* IHp|apply* IHe].
+Qed.    
+
+
+Lemma typing_prf_weaken: forall G E F p T,
+ (E & G) |= p :+ T -> ok (E & F & G) ->  (E & F & G) |= p :+ T.
+Proof.
+  destruct typing_weaken as [Hp _ ].
+  intros;apply* Hp.
+Qed.
+
+Lemma typing_cont_weaken: forall  G E F e T,
+ (E & G) |= e :- T -> ok (E & F & G) ->   (E & F & G) |= e :- T.
+Proof.
+  destruct typing_weaken as [_ (He,_ )].
+  intros;apply* He.
+Qed.
+
+Lemma typing_clos_weaken: forall G E F c,
+c:*(E & G) ->  ok (E & F & G) ->   c:* (E & F & G) .
+Proof.
+  destruct typing_weaken as [_ (_,Hc)].
+  intros;apply* Hc.
+Qed.
+
+(** Typing is preserved by substitution. *)
+
+Lemma typing_prf_not_neg: forall q  U E,
+  E |= q:+ neg U -> False.
+Proof.
+intros q.  
+induction q;intros.
++ admit.
++ admit.
+
+  
+Fixpoint typing_subst_prf F U E p T z q (H:(E & z ~ U & F) |= p:+ T) {struct H}:
+  E |= q :+ U -> (E & F) |= [z ~+> q]+ p :+ T
+with typing_subst_cont F U E e T z q (H:(E & z ~ U & F) |= e:- T ) {struct H}:
+   E |= q :+ U -> (E & F) |= [z ~+> q]- e :- T
+with typing_subst_clos F U E c z q (H:c:* (E & z ~ U & F)) {struct H}:
+   E |= q :+ U -> [z ~+> q]* c :* (E&F).
+Proof.
+  - introv Typq.
+    inductions H;introv; simpl.
+    + case_var.
+      * apply binds_middle_eq_inv in H0.
+        rewrite H0.
+        apply_empty* typing_prf_weaken.
+        assumption.
+      * apply* typing_prf_var.
+        apply* binds_subst.
+    + apply_fresh typing_abs.
+      rewrite* subst_open_prf_prf_var. 
+      apply_ih_bind* H0.
+    + apply_fresh typing_mu.
+      rewrite <- concat_assoc.
+      assert (y \notin L) by intuition.
+      specialize (H y H0).
+      rewrite <- concat_assoc in H.
+      destruct (typing_subst_clos (F & y~neg T) U E c z q H).
+      assumption.
+      apply* typing_closure.
+  - introv Typq.
+    inductions H;introv; simpl.
+    + apply* typing_cont_var.
+      destruct  (binds_middle_inv H0).
+      intuition.
+      destruct* H1.
+      intuition.
+      rewrite <- H4 in Typq.
+      contradict Typq.
+      
+Admitted.
+
+(** Preservation (typing is preserved by reduction). *)
+
+Lemma preservation_result : preservation.
+Proof.
+  introv Typ. gen t'. inductions Typ; introv Red; inversions Red.
+  inversions Typ1. pick_fresh x. rewrite* (@subst_intro x).
+   apply_empty* typing_subst.
+  apply* typing_app. 
+  apply* typing_app.
+Qed.
+
+(** Progress (a well-typed term is either a value or it can 
+  take a step of reduction). *)
+
+Lemma progress_result : progress.
+Proof.
+  introv Typ. lets Typ': Typ. inductions Typ.
+  false* binds_empty_inv. 
+  left*.
+  right. destruct~ IHTyp1 as [Val1 | [t1' Red1]].
+    destruct~ IHTyp2 as [Val2 | [t2' Red2]].
+      inversions Typ1; inversions Val1. exists* (t0 ^^ t2).
+      exists* (trm_app t1 t2'). 
+    exists* (trm_app t1' t2).
+Qed.
+
+
+
